iris/ProofIunlock.v
@@ -437,7 +437,7 @@ Section ProofIunlockMain.
                  eq_refl with "Hbodyp Hvalid Hdep")
       as "(Hvalid & Hdep & Hborp)".
     iDestruct "Hborp" as (sbp) "[Hlvp Hbbackp]".
-    iMod (iref_live_load_au (⊤ ∖ ↑icEscN) k sbp
+    iMod (iref_live_load_au (⊤ ∖ ↑(icEscN .@ k)) k sbp
             ltac:(solve_ndisj) Hk with "Hitbl Hlvp") as (vp) "[Hcellp Hclp]".
     iDestruct (wordw_claim_of (KTR := KT0) 4 (i_ref (ientry k)) (DfracOwn 1) vp
                  ltac:(lia) with "Hcellp") as "#Hclaim0".
@@ -450,7 +450,7 @@ Section ProofIunlockMain.
               (fun v => (⌜0 < bv_unsigned v < 2 ^ 31⌝ ∗
                          i_valid (ientry k) ↦₄ valid_word true ∗
                          ic_deposit cn k (DepShr s dev inum g))%I)
-              (⊤ ∖ ↑minstretN ∖ ↑icEscN ∖ ↑icacheN) b
+              (⊤ ∖ ↑minstretN ∖ ↑(icEscN .@ k) ∖ ↑icacheN) b
               ltac:(nz) ltac:(rdok) ltac:(solve_ndisj)
               with "Hcg Hpc [] [] [Hvalid Hdep]").
     { iApply (iui2_1c with "Htext"). }
@@ -465,7 +465,7 @@ Section ProofIunlockMain.
                    eq_refl with "Hbody Hvalid Hdep")
         as "(Hvalid & Hdep & Hbor)".
       iDestruct "Hbor" as (sb) "[Hlv Hbback]".
-      iMod (iref_live_load_au (⊤ ∖ ↑minstretN ∖ ↑icEscN) k sb
+      iMod (iref_live_load_au (⊤ ∖ ↑minstretN ∖ ↑(icEscN .@ k)) k sb
               ltac:(solve_ndisj) Hk with "Hitbl Hlv") as (v) "[Hcell Hcl]".
       iModIntro. iExists v. iFrame "Hcell". iIntros "Hcell".
       iMod ("Hcl" with "Hcell") as "[%Hb Hlv]".
